theories/c_toy_lang/iris_lang_instantiation.v
@@ -1,0 +1,68 @@
+From stdpp Require Export binders strings.
+From stdpp Require Import gmap.
+From iris.algebra Require Export ofe.
+From iris.program_logic Require Export language ectx_language ectxi_language.
+From iris.heap_lang Require Export locations.
+From iris.prelude Require Import options.
+From melocoton.c_toy_lang Require Export lang.
+
+
+Inductive bogo_head_step (p:program) : expr → state → list unit → expr → state → list expr → Prop :=
+  bogo_obs e1 σ1 e2 σ2 :
+    head_step p e1 σ1 e2 σ2 →
+    bogo_head_step p e1 σ1 [] e2 σ2 [].
+
+Lemma bogo_head_step_elim p e1 σ1 l1 e2 σ2 l2 : 
+  bogo_head_step p e1 σ1 l1 e2 σ2 l2 → head_step p e1 σ1 e2 σ2.
+Proof. by intros []. Qed.
+
+Lemma bogo_head_step_elim' p e1 σ1 l1 e2 σ2 l2 : 
+  bogo_head_step p e1 σ1 l1 e2 σ2 l2 → head_step p e1 σ1 e2 σ2 /\ l1 = [] /\ l2 = [].
+Proof. inversion 1;subst. now repeat split. Qed.
+
+Lemma C_lang_mixin p : EctxiLanguageMixin of_val to_val fill_item (bogo_head_step p).
+Proof.
+  split; apply _ || eauto using bogo_head_step_elim, to_of_val, of_to_val, val_head_stuck,
+    fill_item_val, fill_item_no_val_inj, head_ctx_step_val.
+Qed.
+
+(** Language *)
+Canonical Structure C_ectxi_lang p := EctxiLanguage (C_lang_mixin p).
+Canonical Structure C_ectx_lang p := EctxLanguageOfEctxi (C_ectxi_lang p).
+Canonical Structure C_lang p := LanguageOfEctx (C_ectx_lang p).
+Coercion C_lang : C_lang.program >-> language.
+
+
+(** The following lemma is not provable using the axioms of [ectxi_language].
+The proof requires a case analysis over context items ([destruct i] on the
+last line), which in all cases yields a non-value. To prove this lemma for
+[ectxi_language] in general, we would require that a term of the form
+[fill_item i e] is never a value. *)
+Lemma to_val_fill_some p K e v : to_val (@fill (C_ectxi_lang p) K e) = Some v → K = [] ∧ e = Val v.
+Proof.
+  intro H. destruct K as [|Ki K]; first by apply of_to_val in H. exfalso.
+  assert (to_val e ≠ None) as He.
+  { intro A. by rewrite fill_not_val in H. }
+  assert (∃ w, e = Val w) as [w ->].
+  { destruct e; try done; eauto. }
+  assert (to_val (fill (Ki :: K) (Val w)) = None).
+  { destruct Ki; simpl; apply fill_not_val; done. }
+  by simplify_eq.
+Qed.
+
+Lemma prim_step_to_val_is_head_step p e σ1 κs w σ2 efs :
+  @prim_step (C_ectxi_lang p) e σ1 κs (Val w) σ2 efs → head_step p e σ1 (Val w) σ2.
+Proof.
+  intro H. destruct H as [K e1 e2 H1 H2].
+  assert (to_val (fill K e2) = Some w) as H3; first by rewrite -H2.
+  apply to_val_fill_some in H3 as [-> ->]. subst e. eapply bogo_head_step_elim. apply H.
+Qed.
+
+(** If [e1] makes a head step to a value under some state [σ1] then any head
+ step from [e1] under any other state [σ1'] must necessarily be to a value. *)
+Lemma head_step_to_val p e1 σ1 e2 σ2 σ1' e2' σ2' :
+  head_step p e1 σ1 e2 σ2 →
+  head_step p e1 σ1' e2' σ2' → is_Some (to_val e2) → is_Some (to_val e2').
+Proof.
+  destruct 1; inversion 1; try naive_solver; congruence.
+Qed.
