theories/c_toy_lang/lang_instantiation.v
@@ -1,0 +1,134 @@
+From stdpp Require Export binders strings.
+From stdpp Require Import gmap.
+From iris.algebra Require Export ofe.
+From iris.heap_lang Require Export locations.
+From iris.prelude Require Import options.
+From melocoton.c_toy_lang Require Export iris_lang_instantiation.
+From melocoton.interop Require Import lang_with_calls.
+From melocoton.c_toy_lang Require Export lang metatheory.
+
+Definition of_class (e : mixin_expr_class val) : expr := match e with
+  ExprVal v => Val v
+| ExprCall vf vl => FunCall (Val $ LitV $ LitFunPtr vf) (map Val vl) end.
+#[local] Notation omap f x := (match x with Some v => f v | None => None end).
+Fixpoint unmap_val el := match el with 
+      Val v::er => omap (fun vr => Some (v::vr)) (unmap_val er)
+    | nil => Some nil
+    | _ => None end.
+Definition to_class (e : expr) : option (mixin_expr_class val) := match e with
+  Val v => Some (ExprVal v)
+| FunCall (Val (LitV (LitFunPtr vf))) el => omap (fun l => Some (ExprCall vf l)) (unmap_val el)
+| _ => None end.
+
+Lemma map_unmap_val l : unmap_val (map Val l) = Some l.
+Proof.
+  induction l.
+  - easy.
+  - cbn. rewrite IHl. easy.
+Qed.
+
+Lemma to_of_cancel e : to_class (of_class e) = Some e.
+Proof.
+  destruct e.
+  - easy.
+  - cbn. rewrite map_unmap_val. easy.
+Qed.
+
+Lemma unmap_val_map le lv : unmap_val le = Some lv → map Val lv = le.
+Proof.
+  induction le in lv|-*.
+  - intros H. injection H. intros <-. easy.
+  - cbn. destruct a. 2-13:congruence.
+    destruct (unmap_val le) eqn:Heq. 2:congruence.
+    intros H. injection H. intros <-. cbn. f_equal. now apply IHle.
+Qed.
+
+Lemma of_to_cancel e c : to_class e = Some c → of_class c = e.
+Proof.
+  destruct e; cbn; try congruence.
+  - intros H. injection H. intros <-. easy.
+  - destruct e. 2-13: congruence. destruct v. destruct l. 1-2: congruence.
+    destruct unmap_val eqn:Heq. 2:congruence.
+    intros H. injection H. intros <-. cbn. f_equal. now apply unmap_val_map.
+Qed.
+
+Inductive bogo_head_step' (p:program) : expr → state → expr → state → list expr → Prop :=
+  bogo_obs e1 σ1 e2 σ2 :
+    head_step p e1 σ1 e2 σ2 →
+    bogo_head_step' p e1 σ1 e2 σ2 [].
+
+Lemma bogo_head_step'_elim p e1 σ1 e2 σ2 l2 : 
+  bogo_head_step' p e1 σ1 e2 σ2 l2 → head_step p e1 σ1 e2 σ2.
+Proof. by intros []. Qed.
+
+Lemma bogo_head_step'_elim' p e1 σ1 e2 σ2 l2 : 
+  bogo_head_step' p e1 σ1 e2 σ2 l2 → head_step p e1 σ1 e2 σ2 /\ l2 = [].
+Proof. inversion 1;subst. now repeat split. Qed.
+
+Lemma head_step_no_val p v σ1 e2 σ2 efs :
+  bogo_head_step' p (Val v) σ1 e2 σ2 efs → False.
+Proof.
+  intros H. inversion H; subst. inversion H0.
+Qed.
+
+Lemma fill_class {p:program} (K : list ectx_item) (e:expr) : 
+    is_Some (to_class (ectxi_language.fill K e)) → K = nil ∨ ∃ v, to_class e = Some (ExprVal v).
+Proof.
+  intros [v Hv]. revert v Hv. induction K as [|k1 K] using rev_ind; intros v Hv. 1:now left. right.
+  rewrite fill_app in Hv.
+  destruct k1; cbn in Hv; try congruence.
+  + destruct (ectxi_language.fill K e) eqn:Heq; cbn in Hv; try congruence. destruct v0. destruct l; cbn in Hv; try congruence.
+    revert Hv. edestruct unmap_val eqn:Heq2; try congruence. intros H. injection H. intros <-.
+    cbn in IHK. destruct (IHK _ eq_refl) as [->|Hr].
+    - cbn in Heq. subst. eexists. cbn. reflexivity.
+    - easy.
+  + destruct vf. destruct l; cbn in Hv; try congruence. revert Hv. edestruct unmap_val eqn:Heq; try congruence.
+    intros H. injection H. intros <-. apply unmap_val_map in Heq.
+    assert (In (ectxi_language.fill K e) (map Val l)) as [vv [Hvv' Hvv]]%in_map_iff.
+    1: rewrite Heq; apply in_app_iff; right; now left.
+    destruct (IHK (ExprVal vv)) as [Hl|Hr].
+    - rewrite <- Hvv'. easy.
+    - subst. cbn in *. subst. eexists. cbn. reflexivity.
+    - easy.
+Qed.
+
+Lemma melocoton_lang_mixin_C : 
+  @LanguageMixin expr val function (list ectx_item) state
+                 of_class to_class
+                 nil (fun a b => b++a) (@ectxi_language.fill (C_ectxi_lang (∅:gmap _ _)))
+                 subst_all free_vars
+                 apply_function bogo_head_step'.
+Proof. split.
+  + apply to_of_cancel.
+  + apply of_to_cancel.
+  + apply head_step_no_val.
+  + intros p f vs σ1 e2 σ2 efs. split.
+    - intros H. inversion H; subst. inversion H0; subst. repeat econstructor; [apply H3|].
+      rewrite <- H7. f_equal. eapply map_inj in H2; congruence.
+    - intros ([args ee] & H1 & H2 & -> & ->). econstructor. cbn. by eapply FunCallS.
+  + apply subst_all_empty.
+  + intros e g1 g2. apply subst_all_comp.
+  + intros g1 g2 e. apply subst_all_free_irrel.
+  + intros xs e. apply subst_free_vars.
+  + now intros e.
+  + intros K1 K2 e. now rewrite fill_app.
+  + intros K a b. apply ectx_language.fill_inj.
+  + apply fill_class.
+  + intros p. 
+    change ((@ectxi_language.fill (C_ectxi_lang (∅:gmap _ _)))) with ((@ectxi_language.fill (C_ectxi_lang p))).
+    intros K' K_redec e1' e1_redex σ1 e2 σ2 efs H Heq (Hstep & ->)%bogo_head_step'_elim'.
+    destruct (ectx_language.step_by_val K' K_redec e1' e1_redex σ1 nil e2 σ2 nil H) as [K'' HK''].
+    1: now destruct e1'; cbn in *.
+    1: econstructor; apply Hstep.
+    exists K''. apply HK''.
+  + intros p.
+    change ((@ectxi_language.fill (C_ectxi_lang (∅:gmap _ _)))) with ((@ectxi_language.fill (C_ectxi_lang p))).
+    intros K e σ1 e2 σ2 efs (Hstep & ->)%bogo_head_step'_elim'.
+    change (gmap string function) with program in p.
+    edestruct (ectx_language.head_ctx_step_val K e σ1 nil e2 σ2 nil) as [Hl|Hr].
+    1: econstructor; apply Hstep.
+    1: right; destruct Hl as (v&Hv); exists v; destruct e; cbn in *; congruence.
+    1: left; now rewrite Hr.
+Qed.
+  
+Canonical Structure C_lang_melocoton := Language melocoton_lang_mixin_C.
