theories/interop/lang_with_calls.v
@@ -1,0 +1,1144 @@
+From stdpp Require Import relations strings gmap.
+From iris.algebra Require Import ofe.
+From iris.prelude Require Import options.
+
+Definition thread_id := nat.
+
+Section language_mixin.
+  Context {expr val func ectx state : Type}.
+
+  (** Classifying expressions into values and calls. *)
+  Inductive mixin_expr_class :=
+  | ExprVal (v : val) : mixin_expr_class
+  | ExprCall (fn_name : string) (arg : list val) : mixin_expr_class.
+
+  Context (of_class : mixin_expr_class → expr).
+  Context (to_class : expr → option mixin_expr_class).
+
+  Context (empty_ectx : ectx).
+  Context (comp_ectx : ectx → ectx → ectx).
+  Context (fill : ectx → expr → expr).
+
+  (** Parallel substitution, to define [log_rel] in a language-independent
+      way. *)
+  Context (subst_map : gmap string val → expr → expr).
+  Context (free_vars : expr → gset string).
+
+  (** A program is a map from function names to function bodies. *)
+  Local Notation mixin_prog := (gmap string func).
+
+  Context (apply_func : func → list val → option expr).
+  Context (head_step : mixin_prog → expr → state → expr → state → list expr → Prop).
+
+  Record LanguageMixin := {
+    (** Expression classification *)
+    mixin_to_of_class c : to_class (of_class c) = Some c;
+    mixin_of_to_class e c : to_class e = Some c → of_class c = e;
+
+    (** Reduction behavior of the special classes of expressions *)
+    (** mixin_val_head_step is not an iff because the backward direction is trivial *)
+    mixin_val_head_step p v σ1 e2 σ2 efs :
+      head_step p (of_class (ExprVal v)) σ1 e2 σ2 efs → False;
+    mixin_call_head_step p f vs σ1 e2 σ2 efs :
+      head_step p (of_class (ExprCall f vs)) σ1 e2 σ2 efs ↔
+      ∃ (fn : func),
+        p !! f = Some fn ∧ Some e2 = apply_func fn vs ∧ σ2 = σ1 ∧ efs = [];
+
+    (** Substitution and free variables *)
+    mixin_subst_map_empty e : subst_map ∅ e = e;
+    mixin_subst_map_subst_map xs ys e :
+      subst_map xs (subst_map ys e) = subst_map (ys ∪ xs) e;
+    mixin_subst_map_free_vars (xs1 xs2 : gmap string val) (e : expr) :
+      (∀ x, x ∈ free_vars e → xs1 !! x = xs2 !! x) →
+      subst_map xs1 e = subst_map xs2 e;
+    mixin_free_vars_subst_map xs e :
+      free_vars (subst_map xs e) = free_vars e ∖ (dom xs);
+
+    (** Evaluation contexts *)
+    mixin_fill_empty e : fill empty_ectx e = e;
+    mixin_fill_comp K1 K2 e : fill K1 (fill K2 e) = fill (comp_ectx K1 K2) e;
+    mixin_fill_inj K : Inj (=) (=) (fill K);
+    (* The the things in a class contain only values in redex positions (or the
+       redex is the topmost one). *)
+    mixin_fill_class K e :
+      is_Some (to_class (fill K e)) → K = empty_ectx ∨ ∃ v, to_class e = Some (ExprVal v);
+
+    (** Given a head redex [e1_redex] somewhere in a term, and another
+        decomposition of the same term into [fill K' e1'] such that [e1'] is not
+        a value, then the head redex context is [e1']'s context [K'] filled with
+        another context [K''].  In particular, this implies [e1 = fill K''
+        e1_redex] by [fill_inj], i.e., [e1]' contains the head redex.)
+
+        This implies there can be only one head redex, see
+        [head_redex_unique]. *)
+    mixin_step_by_val p K' K_redex e1' e1_redex σ1 e2 σ2 efs :
+      fill K' e1' = fill K_redex e1_redex →
+      match to_class e1' with Some (ExprVal _) => False | _ => True end →
+      head_step p e1_redex σ1 e2 σ2 efs →
+      ∃ K'', K_redex = comp_ectx K' K'';
+
+    (** If [fill K e] takes a head step, then either [e] is a value or [K] is
+        the empty evaluation context. In other words, if [e] is not a value
+        wrapping it in a context does not add new head redex positions. *)
+    (* FIXME: This is the exact same conclusion as [mixin_fill_class]... is
+       there some pattern or reduncancy here? *)
+    mixin_head_ctx_step_val p K e σ1 e2 σ2 efs :
+      head_step p (fill K e) σ1 e2 σ2 efs → K = empty_ectx ∨ ∃ v, to_class e = Some (ExprVal v);
+  }.
+End language_mixin.
+
+Arguments mixin_expr_class : clear implicits.
+Local Notation mixin_prog func := (gmap string func).
+
+Structure language := Language {
+  expr : Type;
+  val : Type;
+  func : Type;
+  ectx : Type;
+  state : Type;
+
+  of_class : mixin_expr_class val → expr;
+  to_class : expr → option (mixin_expr_class val);
+  empty_ectx : ectx;
+  comp_ectx : ectx → ectx → ectx;
+  fill : ectx → expr → expr;
+  subst_map : gmap string val → expr → expr;
+  free_vars : expr → gset string;
+  apply_func : func → list val → option expr;
+  head_step : mixin_prog func → expr → state → expr → state → list expr → Prop;
+
+  language_mixin :
+    LanguageMixin (val:=val) of_class to_class empty_ectx comp_ectx fill
+      subst_map free_vars apply_func head_step
+}.
+
+Declare Scope expr_scope.
+Bind Scope expr_scope with expr.
+
+Declare Scope val_scope.
+Bind Scope val_scope with val.
+
+Arguments Language {expr _ _ _ _ _ _ _ _ _ _ free_vars apply_func head_step}.
+Arguments of_class {_} _.
+Arguments to_class {_} _.
+Arguments empty_ectx {_}.
+Arguments comp_ectx {_} _ _.
+Arguments fill {_} _ _.
+Arguments subst_map {_}.
+Arguments free_vars {_}.
+Arguments apply_func {_}.
+Arguments head_step {_} _ _ _ _ _ _.
+
+Definition expr_class (Λ : language) := mixin_expr_class Λ.(val).
+(* A [Definition] throws off Coq's "old" ("tactic") unification engine *)
+Notation prog Λ := (mixin_prog Λ.(func)).
+
+Definition to_val {Λ : language} (e : expr Λ) :=
+  match to_class e with
+  | Some (ExprVal v) => Some v
+  | _ => None
+  end.
+Definition of_val {Λ : language} (v : val Λ) := of_class (ExprVal v).
+
+Definition to_call {Λ : language} (e : expr Λ) :=
+  match to_class e with
+  | Some (ExprCall f v) => Some (f, v)
+  | _ => None
+  end.
+Definition of_call {Λ : language} f (v : list (val Λ)) := of_class (ExprCall f v).
+
+(* From an ectx_language, we can construct a language. *)
+Section language.
+  Context {Λ : language}.
+  Implicit Types v : val Λ.
+  Implicit Types vs : list (val Λ).
+  Implicit Types e : expr Λ.
+  Implicit Types c : expr_class Λ.
+  Implicit Types K : ectx Λ.
+  Implicit Types p : prog Λ.
+  Implicit Types efs : list (expr Λ).
+
+  Lemma to_of_class c : to_class (of_class c) = Some c.
+  Proof. apply language_mixin. Qed.
+  Lemma of_to_class e c : to_class e = Some c → of_class c = e.
+  Proof. apply language_mixin. Qed.
+
+  Lemma to_val_of_call f vs : to_val (of_call f vs) = None.
+  Proof. rewrite /to_val /of_call to_of_class. done. Qed.
+  Lemma to_call_of_val v : to_call (of_val v) = None.
+  Proof. rewrite /to_call /of_val to_of_class. done. Qed.
+  Lemma is_val_is_class e : is_Some (to_val e) → is_Some (to_class e).
+  Proof. rewrite /to_val /is_Some. destruct (to_class e) as [[|]|]; naive_solver. Qed.
+  Lemma is_call_is_class e : is_Some (to_call e) → is_Some (to_class e).
+  Proof. rewrite /to_call /is_Some. destruct (to_class e) as [[|]|]; naive_solver. Qed.
+
+  Lemma val_head_step p v σ1 e2 σ2 efs :
+    head_step p (of_class (ExprVal v)) σ1 e2 σ2 efs → False.
+  Proof. apply language_mixin. Qed.
+  Lemma call_head_step p f vs σ1 e2 σ2 efs :
+    head_step p (of_class (ExprCall f vs)) σ1 e2 σ2 efs ↔
+    ∃ fn, p !! f = Some fn ∧ Some e2 = apply_func fn vs ∧ σ2 = σ1 ∧ efs = nil.
+  Proof. apply language_mixin. Qed.
+
+  Lemma subst_map_empty e :
+    subst_map ∅ e = e.
+  Proof. apply language_mixin. Qed.
+  Lemma subst_map_free_vars (xs1 xs2 : gmap string (val Λ)) e :
+    (∀ x, x ∈ free_vars e → xs1 !! x = xs2 !! x) →
+    subst_map xs1 e = subst_map xs2 e.
+  Proof. apply language_mixin. Qed.
+  Lemma subst_map_subst_map xs ys e :
+    subst_map xs (subst_map ys e) = subst_map (ys ∪ xs) e.
+  Proof. apply language_mixin. Qed.
+  Lemma free_vars_subst_map xs e :
+    free_vars (subst_map xs e) = free_vars e ∖ (dom xs).
+  Proof. apply language_mixin. Qed.
+
+  Lemma fill_empty e : fill empty_ectx e = e.
+  Proof. apply language_mixin. Qed.
+  Lemma fill_comp K1 K2 e : fill K1 (fill K2 e) = fill (comp_ectx K1 K2) e.
+  Proof. apply language_mixin. Qed.
+  Global Instance fill_inj K : Inj (=) (=) (fill K).
+  Proof. apply language_mixin. Qed.
+  Lemma fill_class' K e :
+    is_Some (to_class (fill K e)) → K = empty_ectx ∨ ∃ v, to_class e = Some (ExprVal v).
+  Proof. apply language_mixin. Qed.
+  Lemma step_by_val' p K' K_redex e1' e1_redex σ1 e2 σ2 efs :
+      fill K' e1' = fill K_redex e1_redex →
+      match to_class e1' with Some (ExprVal _) => False | _ => True end →
+      head_step p e1_redex σ1 e2 σ2 efs →
+      ∃ K'', K_redex = comp_ectx K' K''.
+  Proof. apply language_mixin. Qed.
+  Lemma head_ctx_step_val' p K e σ1 e2 σ2 efs :
+    head_step p (fill K e) σ1 e2 σ2 efs → K = empty_ectx ∨ ∃ v, to_class e = Some (ExprVal v).
+  Proof. apply language_mixin. Qed.
+
+  Lemma fill_class K e :
+    is_Some (to_class (fill K e)) → K = empty_ectx ∨ is_Some (to_val e).
+  Proof.
+    intros [?|[v Hv]]%fill_class'; first by left. right.
+    rewrite /to_val Hv. eauto.
+  Qed.
+  Lemma step_by_val p K' K_redex e1' e1_redex σ1 e2 σ2 efs :
+      fill K' e1' = fill K_redex e1_redex →
+      to_val e1' = None →
+      head_step p e1_redex σ1 e2 σ2 efs →
+      ∃ K'', K_redex = comp_ectx K' K''.
+  Proof.
+    rewrite /to_val => ? He1'. eapply step_by_val'; first done.
+    destruct (to_class e1') as [[]|]; done.
+  Qed.
+  Lemma head_ctx_step_val p K e σ1 e2 σ2 efs :
+    head_step p (fill K e) σ1 e2 σ2 efs → K = empty_ectx ∨ is_Some (to_val e).
+  Proof.
+    intros [?|[v Hv]]%head_ctx_step_val'; first by left. right.
+    rewrite /to_val Hv. eauto.
+  Qed.
+  Lemma call_head_step_inv p f vs σ1 e2 σ2 efs :
+    head_step p (of_class (ExprCall f vs)) σ1 e2 σ2 efs →
+    ∃ fn, p !! f = Some fn ∧ Some e2 = apply_func fn vs ∧ σ2 = σ1 ∧ efs = nil.
+  Proof. eapply call_head_step. Qed.
+  Lemma call_head_step_intro p f vs fn σ1 er :
+    p !! f = Some fn →
+    Some er = apply_func fn vs →
+    head_step p (of_call f vs) σ1 er σ1 [].
+  Proof. intros ? ?. eapply call_head_step; eexists; eauto. Qed.
+
+  Definition head_reducible (p : prog Λ) (e : expr Λ) (σ : state Λ) :=
+    ∃ e' σ' efs, head_step p e σ e' σ' efs.
+  Definition head_irreducible (p : prog Λ) (e : expr Λ) (σ : state Λ) :=
+    ∀ e' σ' efs, ¬head_step p e σ e' σ' efs.
+  Definition head_stuck (p : prog Λ) (e : expr Λ) (σ : state Λ) :=
+    to_val e = None ∧ head_irreducible p e σ.
+
+  (* All non-value redexes are at the root.  In other words, all sub-redexes are
+     values. *)
+  Definition sub_redexes_are_values (e : expr Λ) :=
+    ∀ K e', e = fill K e' → to_val e' = None → K = empty_ectx.
+
+  Inductive prim_step (p : prog Λ) : expr Λ → state Λ → expr Λ → state Λ → list (expr Λ) → Prop :=
+    Prim_step K e1 e2 σ1 σ2 e1' e2' efs:
+      e1 = fill K e1' → e2 = fill K e2' →
+      head_step p e1' σ1 e2' σ2 efs → prim_step p e1 σ1 e2 σ2 efs.
+
+  Lemma Prim_step' p K e1 σ1 e2 σ2 efs :
+    head_step p e1 σ1 e2 σ2 efs → prim_step p (fill K e1) σ1 (fill K e2) σ2 efs.
+  Proof. econstructor; eauto. Qed.
+
+  Definition reducible (p : prog Λ) (e : expr Λ) (σ : state Λ) :=
+    ∃ e' σ' efs, prim_step p e σ e' σ' efs.
+  Definition irreducible (p : prog Λ) (e : expr Λ) (σ : state Λ) :=
+    ∀ e' σ' efs, ¬prim_step p e σ e' σ' efs.
+  Definition stuck (p : prog Λ) (e : expr Λ) (σ : state Λ) :=
+    to_val e = None ∧ irreducible p e σ.
+  Definition not_stuck (p : prog Λ) (e : expr Λ) (σ : state Λ) :=
+    is_Some (to_val e) ∨ reducible p e σ.
+
+  (** * Some lemmas about this language *)
+  Lemma prim_step_inv p e1 e2 σ1 σ2 efs:
+    prim_step p e1 σ1 e2 σ2 efs →
+    ∃ K e1' e2', e1 = fill K e1' ∧ e2 = fill K e2' ∧ head_step p e1' σ1 e2' σ2 efs.
+  Proof. inversion 1; subst; do 3 eexists; eauto. Qed.
+  Lemma to_of_val v : to_val (of_val v) = Some v.
+  Proof. rewrite /to_val /of_val to_of_class //. Qed.
+  Lemma of_to_val e v : to_val e = Some v → of_val v = e.
+  Proof.
+    rewrite /to_val /of_val => Hval. apply of_to_class.
+    destruct (to_class e) as [[]|]; simplify_option_eq; done.
+  Qed.
+  Lemma of_to_val_flip v e : of_val v = e → to_val e = Some v.
+  Proof. intros <-. by rewrite to_of_val. Qed.
+  Lemma val_head_stuck p e σ e' σ' efs: head_step p e σ e' σ' efs → to_val e = None.
+  Proof.
+    destruct (to_val e) as [v|] eqn:Hval; last done.
+    rewrite -(of_to_val e v) //. intros []%val_head_step.
+  Qed.
+  Lemma fill_val K e : is_Some (to_val (fill K e)) → is_Some (to_val e).
+  Proof.
+    intros Hval. destruct (fill_class K e) as [HK|He].
+    - apply is_val_is_class. done.
+    - subst K. move: Hval. rewrite fill_empty. done.
+    - done.
+  Qed.
+  Lemma val_stuck p e σ e' σ' efs: prim_step p e σ e' σ' efs → to_val e = None.
+  Proof.
+    intros (?&?&? & -> & -> & ?%val_head_stuck)%prim_step_inv.
+    apply eq_None_not_Some. by intros ?%fill_val%eq_None_not_Some.
+  Qed.
+
+  Lemma to_of_call f vs : to_call (of_call f vs) = Some (f, vs).
+  Proof. rewrite /to_call /of_call to_of_class //. Qed.
+  Lemma of_to_call e f vs : to_call e = Some (f, vs) → of_call f vs = e.
+  Proof.
+    rewrite /to_call /of_call => Hval. apply of_to_class.
+    destruct (to_class e) as [[] | ]; simplify_option_eq; done.
+  Qed.
+  Lemma of_to_call_flip f vs e : of_call f vs = e → to_call e = Some (f, vs).
+  Proof. intros <-. apply to_of_call. Qed.
+
+  Lemma not_reducible p e σ : ¬reducible p e σ ↔ irreducible p e σ.
+  Proof. unfold reducible, irreducible. naive_solver. Qed.
+  Lemma reducible_not_val p e σ : reducible p e σ → to_val e = None.
+  Proof. intros (?&?&?&?); eauto using val_stuck. Qed.
+  Lemma val_irreducible p e σ : is_Some (to_val e) → irreducible p e σ.
+  Proof. intros [??] ?? ??%val_stuck. by destruct (to_val e). Qed.
+  Global Instance of_val_inj : Inj (=) (=) (@of_val Λ).
+  Proof. by intros v v' Hv; apply (inj Some); rewrite -!to_of_val Hv. Qed.
+  Lemma not_not_stuck p e σ : ¬not_stuck p e σ ↔ stuck p e σ.
+  Proof.
+    rewrite /stuck /not_stuck -not_eq_None_Some -not_reducible.
+    destruct (decide (to_val e = None)); naive_solver.
+  Qed.
+
+  Lemma fill_not_val K e : to_val e = None → to_val (fill K e) = None.
+  Proof. rewrite !eq_None_not_Some. eauto using fill_val. Qed.
+
+  Lemma not_head_reducible p e σ : ¬head_reducible p e σ ↔ head_irreducible p e σ.
+  Proof. unfold head_reducible, head_irreducible. naive_solver. Qed.
+
+  Lemma subst_map_closed xs e :
+    free_vars e = ∅ →
+    subst_map xs e = e.
+  Proof.
+    intros Hclosed.
+    trans (subst_map ∅ e).
+    - apply subst_map_free_vars. rewrite Hclosed. done.
+    - apply subst_map_empty.
+  Qed.
+
+  (** The decomposition into head redex and context is unique.
+
+      In all sensible instances, [comp_ectx K' empty_ectx] will be the same as
+      [K'], so the conclusion is [K = K' ∧ e = e'], but we do not require a law
+      to actually prove that so we cannot use that fact here. *)
+  Lemma head_redex_unique p K K' e e' σ :
+    fill K e = fill K' e' →
+    head_reducible p e σ →
+    head_reducible p e' σ →
+    K = comp_ectx K' empty_ectx ∧ e = e'.
+  Proof.
+    intros Heq (e2 & σ2 & efs & Hred) (e2' & σ2' & efs' & Hred').
+    edestruct (step_by_val p K' K e' e) as [K'' HK];
+      [by eauto using val_head_stuck..|].
+    subst K. move: Heq. rewrite -fill_comp. intros <-%(inj (fill _)).
+    destruct (head_ctx_step_val _ _ _ _ _ _ _ Hred') as [HK''|[]%not_eq_None_Some].
+    - subst K''. rewrite fill_empty. done.
+    - by eapply val_head_stuck.
+  Qed.
+
+  Lemma head_prim_step p e1 σ1 e2 σ2 efs :
+    head_step p e1 σ1 e2 σ2 efs → prim_step p e1 σ1 e2 σ2 efs.
+  Proof. apply Prim_step with empty_ectx; by rewrite ?fill_empty. Qed.
+
+  Lemma head_step_not_stuck p e σ e' σ' efs:
+    head_step p e σ e' σ' efs → not_stuck p e σ.
+  Proof. rewrite /not_stuck /reducible /=. eauto 10 using head_prim_step. Qed.
+
+  Lemma fill_prim_step p K e1 σ1 e2 σ2 efs :
+    prim_step p e1 σ1 e2 σ2 efs → prim_step p (fill K e1) σ1 (fill K e2) σ2 efs.
+  Proof.
+    intros (K' & e1' & e2' & -> & -> & ?) % prim_step_inv.
+    rewrite !fill_comp. by econstructor.
+  Qed.
+  Lemma fill_reducible p K e σ : reducible p e σ → reducible p (fill K e) σ.
+  Proof.
+    intros (e'&σ'&efs&?). exists (fill K e'), σ', efs. by apply fill_prim_step.
+  Qed.
+  Lemma head_prim_reducible p e σ : head_reducible p e σ → reducible p e σ.
+  Proof. intros (e'&σ'&efs&?). eexists e', σ', efs. by apply head_prim_step. Qed.
+  Lemma head_prim_fill_reducible p e K σ :
+    head_reducible p e σ → reducible p (fill K e) σ.
+  Proof. intro. by apply fill_reducible, head_prim_reducible. Qed.
+  Lemma head_prim_irreducible p e σ : irreducible p e σ → head_irreducible p e σ.
+  Proof.
+    rewrite -not_reducible -not_head_reducible. eauto using head_prim_reducible.
+  Qed.
+
+  Lemma prim_head_step p e σ e' σ' efs:
+    prim_step p e σ e' σ' efs → sub_redexes_are_values e → head_step p e σ e' σ' efs.
+  Proof.
+    intros Hprim ?. destruct (prim_step_inv _ _ _ _ _ _ Hprim) as (K & e1' & e2' & -> & -> & Hstep).
+    assert (K = empty_ectx) as -> by eauto 10 using val_head_stuck.
+    rewrite !fill_empty /head_reducible; eauto.
+  Qed.
+  Lemma prim_head_reducible p e σ :
+    reducible p e σ → sub_redexes_are_values e → head_reducible p e σ.
+  Proof. intros (e'&σ'&efs&Hprim) ?. do 3 eexists; by eapply prim_head_step. Qed.
+  Lemma prim_head_irreducible p e σ :
+    head_irreducible p e σ → sub_redexes_are_values e → irreducible p e σ.
+  Proof.
+    rewrite -not_reducible -not_head_reducible. eauto using prim_head_reducible.
+  Qed.
+
+  Lemma head_stuck_stuck p e σ :
+    head_stuck p e σ → sub_redexes_are_values e → stuck p e σ.
+  Proof.
+    intros [] ?. split; first done. by apply prim_head_irreducible.
+  Qed.
+
+  Lemma head_reducible_prim_step_ctx p K e1 σ1 e2 σ2 efs :
+    head_reducible p e1 σ1 →
+    prim_step p (fill K e1) σ1 e2 σ2 efs →
+    ∃ e2', e2 = fill K e2' ∧ head_step p e1 σ1 e2' σ2 efs.
+  Proof.
+    intros (e2''&σ2''&efs'&HhstepK) (K' & e1' & e2' & HKe1 & -> & Hstep) % prim_step_inv.
+    edestruct (step_by_val p K) as [K'' ?];
+      eauto using val_head_stuck; simplify_eq/=.
+    rewrite -fill_comp in HKe1; simplify_eq.
+    exists (fill K'' e2'). rewrite fill_comp; split; first done.
+    apply head_ctx_step_val in HhstepK as [?|[v ?]]; simplify_eq.
+    - by rewrite !fill_empty.
+    - apply val_head_stuck in Hstep; simplify_eq.
+  Qed.
+
+  Lemma head_reducible_prim_step p e1 σ1 e2 σ2 efs :
+    head_reducible p e1 σ1 →
+    prim_step p e1 σ1 e2 σ2 efs →
+    head_step p e1 σ1 e2 σ2 efs.
+  Proof.
+    intros.
+    edestruct (head_reducible_prim_step_ctx p empty_ectx) as (?&?&?);
+      rewrite ?fill_empty; eauto.
+    by simplify_eq; rewrite fill_empty.
+  Qed.
+
+  Lemma fill_stuck (P : prog Λ) e σ K : stuck P e σ → stuck P (fill K e) σ.
+  Proof.
+    intros Hstuck; split.
+    + apply fill_not_val, Hstuck.
+    + intros e'' σ'' efs (K_redex &e1 &e2 &Heq &-> &Hhead)%prim_step_inv.
+      edestruct (step_by_val P K K_redex _ _ _ _ _ _ Heq ltac:(apply Hstuck) Hhead) as (K'' & ->).
+      rewrite -fill_comp in Heq. apply fill_inj in Heq as ->.
+      eapply (proj2 Hstuck). econstructor; eauto.
+  Qed.
+
+  Lemma fill_not_stuck (P : prog Λ) e σ K : not_stuck P (fill K e) σ → not_stuck P e σ.
+  Proof.
+    intros [Hval | Hred].
+    - left. by eapply fill_val.
+    - destruct Hred as (e' & σ' & efs & (K_redex &e1 &e2 &Heq &-> &Hhead)%prim_step_inv).
+      destruct (decide (to_val e = None)) as [Hnval | Hval]; first last.
+      { left. destruct (to_val e) as [v | ]; by eauto. }
+      edestruct (step_by_val P K K_redex _ _ _ _ _ _ Heq Hnval Hhead) as (K'' & ->).
+      rewrite -fill_comp in Heq. apply fill_inj in Heq as ->.
+      right. eexists _, _, _. econstructor; eauto.
+  Qed.
+
+  Lemma prim_step_call_inv p K f vs e' σ σ' efs :
+    prim_step p (fill K (of_call f vs)) σ e' σ' efs →
+    ∃ er fn, Some er = apply_func fn vs ∧ p !! f = Some fn ∧ e' = fill K er ∧ σ' = σ ∧ efs = [].
+  Proof.
+    intros (K' & e1 & e2 & Hctx & -> & Hstep)%prim_step_inv.
+    eapply step_by_val in Hstep as H'; eauto; last apply to_val_of_call.
+    destruct H' as [K'' Hctx']; subst K'.
+    rewrite -fill_comp in Hctx. eapply fill_inj in Hctx.
+    destruct (fill_class K'' e1) as [->|Hval].
+    - apply is_call_is_class. erewrite of_to_call_flip; eauto.
+    - rewrite fill_empty in Hctx. subst e1. exists e2.
+      apply call_head_step_inv in Hstep as (fn & ? & -> & -> & ->).
+      exists fn. rewrite -fill_comp fill_empty. naive_solver.
+    - unfold is_Some in Hval. erewrite val_head_stuck in Hval; naive_solver.
+  Qed.
+
+  Lemma val_prim_step p v σ e' σ' efs :
+   ¬ prim_step p (of_val v) σ e' σ' efs.
+  Proof.
+    intros (K & e1' & e2' & Heq & -> & Hstep') % prim_step_inv.
+    edestruct (fill_val K e1') as (v1''& ?).
+    { rewrite -Heq. rewrite to_of_val. by exists v. }
+    eapply val_head_step.
+    erewrite <-(of_to_val e1') in Hstep'; eauto.
+  Qed.
+
+  Lemma fill_reducible_prim_step p e e' σ σ' K efs :
+    reducible p e σ → prim_step p (fill K e) σ e' σ' efs → ∃ e'', e' = fill K e'' ∧ prim_step p e σ e'' σ' efs.
+  Proof.
+    intros (e1 & σ1 & efs' & (K'' & e1'' & e2'' & ->  & -> & Hhead) % prim_step_inv) Hprim.
+    rewrite fill_comp in Hprim.
+    eapply head_reducible_prim_step_ctx in Hprim as (e1' & -> & Hhead'); last by rewrite /head_reducible; eauto.
+    eexists. rewrite -fill_comp; by eauto using Prim_step'.
+  Qed.
+
+  (** Lifting of steps to thread pools *)
+  Definition tpool Λ := list (expr Λ).
+  Implicit Types (T: tpool Λ).  (* thread pools *)
+  Implicit Types (I J: list nat).       (* traces *)
+  Implicit Types (O: gset nat).       (* trace sets *)
+
+  Inductive pool_step (p: prog Λ): tpool Λ → state Λ → nat → tpool Λ → state Λ → Prop :=
+    | Pool_step i T_l e e' T_r efs σ σ':
+        prim_step p e σ e' σ' efs →
+        i = length T_l →
+        pool_step p (T_l ++ e :: T_r) σ i (T_l ++ e' :: T_r ++ efs) σ'.
+
+  Inductive pool_steps (p: prog Λ): tpool Λ → state Λ → list nat → tpool Λ → state Λ → Prop :=
+    | Pool_steps_refl T σ: pool_steps p T σ [] T σ
+    | Pool_steps_step T T' T'' σ σ' σ'' i I:
+      pool_step p T σ i T' σ' →
+      pool_steps p T' σ' I T'' σ'' →
+      pool_steps p T σ (i:: I) T'' σ''.
+
+
+  Lemma pool_step_iff p T σ i T' σ':
+    pool_step p T σ i T' σ' ↔
+    (∃ e e' efs, prim_step p e σ e' σ' efs ∧ T !! i = Some e ∧ T' = <[i := e']> T ++ efs).
+  Proof.
+    split.
+    - destruct 1 as [i T_l e e' T_r efs σ σ' Hstep Hlen]; subst.
+      exists e, e', efs. split; first done.
+      rewrite list_lookup_middle; last done.
+      split; first done.
+      replace (length T_l) with (length T_l + 0) by lia.
+      rewrite insert_app_r; simpl.
+      by rewrite -app_assoc.
+    - intros (e & e' & efs & Hstep & Hlook & ->).
+      replace T with (take i T ++ e :: drop (S i) T); last by eapply take_drop_middle.
+      assert (i = length (take i T)).
+      { rewrite take_length_le; first lia. eapply lookup_lt_Some in Hlook. lia. }
+      replace i with (length (take i T) + 0) at 4 by lia.
+      rewrite insert_app_r. simpl.
+      rewrite -app_assoc; simpl.
+      econstructor; auto.
+  Qed.
+
+  Lemma pool_step_value_preservation p v T σ i j T' σ':
+    pool_step p T σ j T' σ' →
+    T !! i = Some (of_val v) →
+    T' !! i = Some (of_val v).
+  Proof.
+    rewrite pool_step_iff.
+    destruct 1 as (e1 & e2 & efs & Hstep & Hpre & Hpost).
+    intros Hlook. destruct (decide (i = j)); subst.
+    - pose proof val_prim_step. by naive_solver.
+    - eapply lookup_app_l_Some.
+      rewrite list_lookup_insert_ne; done.
+  Qed.
+
+  Lemma pool_steps_value_preservation p v T σ i J T' σ':
+    pool_steps p T σ J T' σ' →
+    T !! i = Some (of_val v) →
+    T' !! i = Some (of_val v).
+  Proof.
+    induction 1; eauto using pool_step_value_preservation.
+  Qed.
+
+  Lemma pool_steps_single p T σ i T' σ':
+    pool_step p T σ i T' σ' ↔
+    pool_steps p T σ [i] T' σ'.
+  Proof.
+    split.
+    - intros Hstep; eauto using pool_steps.
+    - inversion 1 as [|????????? Hsteps]. subst; inversion Hsteps; by subst.
+  Qed.
+
+  Lemma pool_steps_trans p T T' T'' σ σ' σ'' I J:
+    pool_steps p T σ I T' σ' →
+    pool_steps p T' σ' J T'' σ'' →
+    pool_steps p T σ (I ++ J) T'' σ''.
+  Proof.
+    induction 1; simpl; eauto using pool_steps.
+  Qed.
+
+
+  (** Threads in a thread pool *)
+  Definition threads T :=
+    list_to_set (C := gset nat) (seq 0 (length T)).
+
+  Lemma threads_spec T i:
+    i ∈ threads T ↔ ∃ e, T !! i = Some e.
+  Proof.
+    rewrite elem_of_list_to_set elem_of_seq.
+    split.
+    - intros [_ Hlt]. eapply lookup_lt_is_Some_2. lia.
+    - intros ? % lookup_lt_is_Some_1. lia.
+  Qed.
+
+  Lemma threads_insert T i e:
+    threads T ⊆ threads (<[i:=e]> T).
+  Proof.
+    intros j [e' Hlook]%threads_spec.
+    eapply threads_spec.
+    destruct (decide (i = j)).
+    - subst; exists e.
+      eapply list_lookup_insert, lookup_lt_Some, Hlook.
+    - rewrite list_lookup_insert_ne; last done. by exists e'.
+  Qed.
+
+  Lemma threads_app T T':
+    threads T ⊆ threads (T ++ T').
+  Proof.
+    intros j (e & Hlook)%threads_spec.
+    eapply threads_spec. exists e.
+    eapply lookup_app_l_Some, Hlook.
+  Qed.
+
+  (* a prim_step does the following mutation to the thread pool *)
+  Lemma threads_prim_step e' T' i T :
+    threads T ⊆ threads (<[i := e']> T ++ T').
+  Proof.
+    etrans; last eapply threads_app.
+    eapply threads_insert.
+  Qed.
+
+  Lemma threads_pool_step p T σ i T' σ' :
+    pool_step p T σ i T' σ' →
+    threads T ⊆ threads T'.
+  Proof.
+    rewrite pool_step_iff; intros (e & e' & efs & Hstep & Hlook & ->).
+    eapply threads_prim_step.
+  Qed.
+
+  Lemma threads_pool_steps p T σ I T' σ' :
+    pool_steps p T σ I T' σ' →
+    threads T ⊆ threads T'.
+  Proof.
+    induction 1; first done.
+    etrans; first eapply threads_pool_step; eauto.
+  Qed.
+
+  (** Reaching Stuck States/Safety *)
+  (* a thread pool has undefined behavior, if one of its threads has undefined behavior. *)
+  Definition not_stuck_pool p T σ := ∀ e i, T !! i = Some e → not_stuck p e σ.
+  Definition pool_safe p T σ := ∀ T' σ' I, pool_steps p T σ I T' σ' → not_stuck_pool p T' σ'.
+  Definition stuck_pool p T σ := (∃ e i, T !! i = Some e ∧ stuck p e σ).
+  Definition pool_reach_stuck p T σ :=
+    ∃ T' σ' I, pool_steps p T σ I T' σ' ∧ stuck_pool p T' σ'.
+
+  Lemma stuck_pool_not_not_stuck_pool p T σ :
+    stuck_pool p T σ → ¬ not_stuck_pool p T σ.
+  Proof.
+    intros (e & i & Hlookup & [Hnval Hirred]) Hnot.
+    apply Hnot in Hlookup as [Hval | Hred].
+    - rewrite Hnval in Hval. destruct Hval as [? [=]].
+    - apply not_reducible in Hirred. done.
+  Qed.
+
+  Lemma pool_reach_stuck_not_safe p T σ :
+    pool_reach_stuck p T σ → ¬ pool_safe p T σ.
+  Proof.
+    intros (T' & σ' & I & Hsteps & Hstuck) Hsafe.
+    apply Hsafe in Hsteps. eapply stuck_pool_not_not_stuck_pool; done.
+  Qed.
+
+  Lemma pool_step_singleton p e σ i σ' T:
+    pool_step p [e] σ i T σ' ↔
+    (∃ e' efs, prim_step p e σ e' σ' efs ∧ T = e' :: efs ∧ i = 0).
+  Proof.
+    rewrite pool_step_iff. destruct i; simpl; naive_solver.
+  Qed.
+
+  Lemma pool_steps_values p T σ I T' σ' :
+    pool_steps p T σ I T' σ' →
+    (∀ e, e ∈ T → is_Some (to_val e)) →
+    T' = T ∧ σ = σ' ∧ I = [].
+  Proof.
+    destruct 1 as [|T T' T'' σ σ' σ'' i I Hstep Hsteps]; eauto.
+    intros Hvals.
+    eapply pool_step_iff in Hstep as (e & e' & efs & Hstep & Hlook & Hupd).
+    feed pose proof (Hvals e) as Irr; first by eapply elem_of_list_lookup_2.
+    exfalso; eapply val_irreducible; eauto.
+  Qed.
+
+  Lemma pool_step_fill_context p e K i j σ σ' T T':
+    pool_step p T σ j T' σ' →
+    T !! i = Some e →
+    ∃ e', T' !! i = Some e' ∧
+    pool_step p (<[i := fill K e]> T) σ j (<[i := fill K e']> T') σ'.
+  Proof.
+    rewrite pool_step_iff; intros (e1 & e2 & efs & Hprim & Hlook & Hupd) Hlook1.
+    destruct (decide (i = j)).
+    - subst. assert (<[j:=e2]> T !! j = Some e2) as Hlook2.
+      { eapply list_lookup_insert, lookup_lt_Some, Hlook. }
+      exists e2; split; first eapply lookup_app_l_Some, Hlook2.
+      rewrite insert_app_l; last by eapply lookup_lt_Some, Hlook2.
+      rewrite list_insert_insert. assert (e1 = e) as -> by naive_solver.
+      eapply pool_step_iff; exists (fill K e), (fill K e2), efs.
+      split; first by eapply fill_prim_step.
+      split; first eapply list_lookup_insert, lookup_lt_Some, Hlook.
+      by rewrite list_insert_insert.
+    - exists e. rewrite Hupd.
+      rewrite (lookup_app_l_Some _ _ _ e);
+        last by rewrite list_lookup_insert_ne //.
+      rewrite insert_app_l;
+        last (eapply lookup_lt_Some; rewrite list_lookup_insert_ne //).
+      split; first done.
+      rewrite list_insert_commute //.
+      eapply pool_step_iff; exists e1, e2, efs.
+      split; first done.
+      split; first rewrite list_lookup_insert_ne //.
+      done.
+  Qed.
+
+  Lemma pool_steps_fill_context p e K i I σ σ' T T':
+    pool_steps p T σ I T' σ' →
+    T !! i = Some e →
+    ∃ e', T' !! i = Some e' ∧
+    pool_steps p (<[i := fill K e]> T) σ I (<[i := fill K e']> T') σ'.
+  Proof.
+    induction 1 as [T σ|T T' T'' σ σ' σ'' j I Hstep Hsteps IH] in e.
+    - eauto 10 using pool_steps.
+    - intros Hlook.
+      eapply pool_step_fill_context in Hlook as (e' & Hlook' & Hstep'); last done.
+      eapply IH in Hlook' as (e'' & Hlook'' & Hstep'').
+      eauto 10 using pool_steps.
+  Qed.
+
+  Lemma pool_steps_safe p T I T' σ σ':
+    pool_steps p T σ I T' σ' → pool_safe p T σ → pool_safe p T' σ'.
+  Proof.
+    intros Hs1 Hsafe T'' σ'' I' Hsteps. eapply Hsafe. eapply pool_steps_trans; done.
+  Qed.
+
+  Lemma pool_safe_insert_fill p T i e σ K :
+    T !! i = Some e →
+    pool_safe p (<[i := fill K e]> T) σ →
+    pool_safe p T σ.
+  Proof.
+    intros Hlook Hsafe T' σ' I Hsteps.
+    eapply (pool_steps_fill_context _ _ K) in Hsteps as (e' & Hlook' & Hsteps); last done.
+    intros e'' j He''.
+    destruct (decide (i = j)) as [-> | Hneq].
+    - assert (e'' = e') as -> by naive_solver.
+      eapply fill_not_stuck. eapply Hsafe; first done.
+      eapply list_lookup_insert, lookup_lt_Some, Hlook'.
+    - eapply Hsafe; first done. rewrite list_lookup_insert_ne //.
+  Qed.
+
+  Lemma fill_reach_stuck_pool p T i e σ K :
+    T !! i = Some e →
+    pool_reach_stuck p T σ →
+    pool_reach_stuck p (<[i := fill K e]> T) σ.
+  Proof.
+    intros Hlook (T' & σ' & I & Hsteps & Hstuck).
+    eapply (pool_steps_fill_context _ _ K) in Hsteps as (e' & Hlook' & Hsteps); last done.
+    exists (<[i:=fill K e']> T'), σ', I; split; first done.
+    destruct Hstuck as (e'' & j & Hlook'' & Hstuck).
+    destruct (decide (i = j)).
+    - subst. exists (fill K e'), j. assert (e'' = e') as -> by naive_solver.
+      split; first eapply list_lookup_insert, lookup_lt_Some, Hlook'.
+      eapply fill_stuck, Hstuck.
+    - exists e'', j. rewrite list_lookup_insert_ne //.
+  Qed.
+
+  Lemma pool_steps_reach_stuck p T I T' σ σ':
+    pool_steps p T σ I T' σ' → pool_reach_stuck p T' σ' → pool_reach_stuck p T σ.
+  Proof.
+    intros H (e'' & σ'' & J & Hstep & Hstuck).
+    exists e'', σ'', (I ++ J). split; last assumption.
+    by eapply pool_steps_trans.
+  Qed.
+
+  Lemma pool_safe_call_in_prg p K T T' i I σ σ' f vs:
+    pool_safe p T σ →
+    pool_steps p T σ I T' σ' →
+    T' !! i = Some (fill K (of_call f vs)) →
+    ∃ fn', p !! f = Some fn'.
+  Proof.
+    destruct (p !! f) as [fn'|] eqn: Hloook; first by eauto.
+    intros Hsafe Hsteps Hlook. exfalso.
+    apply Hsafe in Hsteps. apply Hsteps in Hlook.
+    apply fill_not_stuck in Hlook as [Hval | Hred].
+    - rewrite to_val_of_call in Hval. destruct Hval as [? [=]].
+    - destruct Hred as (e'' & σ'' & efs & Hstep).
+      pose proof (prim_step_call_inv p empty_ectx f vs e'' σ' σ'' efs) as Hinv.
+      rewrite fill_empty in Hinv.
+      eapply Hinv in Hstep as (x_f & e_f & _ & Hprg & _). naive_solver.
+  Qed.
+
+  (** Some theory for sub-pools
+      (needed for the single-thread "reach stuck" further down) *)
+  Lemma pool_step_sub_pool p T1 T1' σ i T2 σ' :
+    pool_step p T1 σ i T1' σ' →
+    T1 ⊆+ T2 →
+    ∃ T2' j, T1' ⊆+ T2' ∧ pool_step p T2 σ j T2' σ'.
+  Proof.
+    intros (e & e' & efs & Hstep & Hlook & ->)%pool_step_iff Hsub.
+    eapply lookup_submseteq in Hsub as Hidx; last done.
+    destruct Hidx as (j & Hlook').
+    exists (<[j := e']> T2 ++ efs), j.
+    split; last (apply pool_step_iff; eauto 10).
+    eapply submseteq_app; last done.
+    eapply submseteq_insert; eauto.
+  Qed.
+
+  Lemma pool_steps_sub_pool p T1 T1' σ I T2 σ' :
+    pool_steps p T1 σ I T1' σ' →
+    T1 ⊆+ T2 →
+    ∃ T2' J, T1' ⊆+ T2' ∧ pool_steps p T2 σ J T2' σ'.
+  Proof.
+    induction 1 as [|T1 T1' T1'' σ σ' σ'' i I Hstep Hsteps IH] in T2; first by eauto using pool_steps.
+    intros Hsub; eapply pool_step_sub_pool in Hstep as (T2' & j & Hpool & Hstep); last done.
+    edestruct IH as (? & ? & ? & ?); eauto 10 using pool_steps.
+  Qed.
+
+  Lemma pool_safe_sub_pool p T1 T2 σ :
+    pool_safe p T2 σ →
+    T1 ⊆+ T2 →
+    pool_safe p T1 σ.
+  Proof.
+    intros Hsafe Hsub T' σ' I Hsteps e i He.
+    eapply pool_steps_sub_pool in Hsteps as (T2' & J & Hsub' & Hsteps'); last done.
+    eapply lookup_submseteq in Hsub' as (j & Hlook'); last done.
+    eapply Hsafe; done.
+  Qed.
+
+  Lemma pool_reach_stuck_sub_pool p T1 T2 σ:
+    pool_reach_stuck p T1 σ →
+    T1 ⊆+ T2 →
+    pool_reach_stuck p T2 σ.
+  Proof.
+    intros (T1' & σ' & I & Hsteps & Hstuck) Hsub.
+    eapply pool_steps_sub_pool in Hsteps as (T2' & J & Hsub' & Hsteps'); last done.
+    exists T2', σ', J; split; first done.
+    destruct Hstuck as (e & i & Hlook & Hstuck).
+    eapply lookup_submseteq in Hsub' as (j & Hlook'); last done.
+    exists e, j; split; eauto.
+  Qed.
+
+  (** we define the one-thread versions of the above pool notions and lemmas *)
+  Definition reach_stuck p e σ := pool_reach_stuck p [e] σ.
+  Definition safe p e σ := pool_safe p [e] σ.
+  Definition step_no_fork p e σ e' σ' := prim_step p e σ e' σ' [].
+  Inductive steps_no_fork (p: prog Λ): expr Λ → state Λ → expr Λ → state Λ → Prop :=
+    | no_forks_refl e σ: steps_no_fork p e σ e σ
+    | no_forks_step e e' e'' σ σ' σ'':
+      step_no_fork p e σ e' σ' →
+      steps_no_fork p e' σ' e'' σ'' →
+      steps_no_fork p e σ e'' σ''.
+
+  Lemma pool_safe_threads_safe p T σ i e:
+    pool_safe p T σ →
+    T !! i = Some e →
+    safe p e σ.
+  Proof.
+    intros Hsafe Hlook. eapply pool_safe_sub_pool; first done.
+    eapply singleton_submseteq_l.
+    apply elem_of_list_lookup. eauto.
+  Qed.
+
+  Lemma pool_reach_stuck_reach_stuck p e σ i T:
+    reach_stuck p e σ →
+    T !! i = Some e →
+    pool_reach_stuck p T σ.
+  Proof.
+    intros Hstuck Hlook.
+    eapply pool_reach_stuck_sub_pool; first apply Hstuck.
+    eapply singleton_submseteq_l.
+    apply elem_of_list_lookup. eauto.
+  Qed.
+
+  Lemma stuck_reach_stuck P e σ:
+    stuck P e σ → reach_stuck P e σ.
+  Proof. intros Hs; exists [e], σ, []. split; [constructor|]. by eexists _, 0. Qed.
+
+  Lemma fill_no_fork p e e' σ σ' K :
+    step_no_fork p e σ e' σ' → step_no_fork p (fill K e) σ (fill K e') σ'.
+  Proof.
+    intros ?; by eapply fill_prim_step.
+  Qed.
+
+  Lemma fill_no_forks p e e' σ σ' K :
+    steps_no_fork p e σ e' σ' → steps_no_fork p (fill K e) σ (fill K e') σ'.
+  Proof.
+    induction 1; eauto using steps_no_fork, fill_no_fork.
+  Qed.
+
+  Lemma fill_reach_stuck p e σ K :
+    reach_stuck p e σ → reach_stuck p (fill K e) σ.
+  Proof.
+    intros Hreach; eapply (fill_reach_stuck_pool _ [e] 0); done.
+  Qed.
+
+  Lemma fill_safe p e σ K :
+    safe p (fill K e) σ → safe p e σ.
+  Proof.
+    intros Hsafe. eapply (pool_safe_insert_fill _ [e] 0); done.
+  Qed.
+
+  Lemma no_forks_pool_steps_single_thread p e σ e' σ':
+    steps_no_fork p e σ e' σ' →
+    (∃ I, pool_steps p [e] σ I [e'] σ').
+  Proof.
+    induction 1 as [|e e' e'' σ σ' σ'' step_no_fork _ IH]; eauto using pool_steps.
+    destruct IH as (I & Hsteps). exists (0 :: I).
+    econstructor; first eapply pool_step_singleton; eauto 10.
+  Qed.
+
+  Lemma prim_step_pool_step T i p e σ e' σ' efs :
+    prim_step p e σ e' σ' efs →
+    T !! i = Some e →
+    pool_step p T σ i (<[i := e']> T ++ efs) σ'.
+  Proof.
+    intros ??. eapply pool_step_iff. eauto 10.
+  Qed.
+
+  Lemma no_fork_pool_step T i p e σ e' σ' :
+    step_no_fork p e σ e' σ' →
+    T !! i = Some e →
+    pool_step p T σ i (<[i := e']> T) σ'.
+  Proof.
+    intros Hnf Hlook. eapply prim_step_pool_step in Hnf; eauto.
+    by rewrite right_id in Hnf.
+  Qed.
+
+  Lemma no_forks_pool_steps T i p e σ e' σ':
+    steps_no_fork p e σ e' σ' →
+    T !! i = Some e →
+    ∃ I, pool_steps p T σ I (<[i := e']> T) σ' ∧ ((list_to_set I: gset nat) ⊆ {[i]}).
+  Proof.
+    induction 1 as [|e e' e'' σ σ' σ'' Hstep Hsteps IH] in T; intros Hlook.
+    - exists []. rewrite list_insert_id //. split; first constructor.
+      set_solver.
+    - eapply no_fork_pool_step in Hstep; last done.
+      destruct (IH (<[i := e']> T)) as (I & Hsteps' & Hsub').
+      { eapply list_lookup_insert, lookup_lt_Some, Hlook. }
+      exists (i :: I). split; last set_solver.
+      rewrite list_insert_insert in Hsteps'.
+      econstructor; done.
+  Qed.
+
+
+  Lemma no_forks_then_prim_step_pool_steps T i p e σ e' σ' e'' σ'' efs:
+    steps_no_fork p e σ e' σ' →
+    prim_step p e' σ' e'' σ'' efs →
+    T !! i = Some e →
+    ∃ I, pool_steps p T σ I (<[i := e'']> T ++ efs) σ'' ∧ ((list_to_set I: gset nat) = {[i]}).
+  Proof.
+    intros Hnfs Hprim Hlook. eapply no_forks_pool_steps in Hnfs as (I & Hsteps & Hsub); last done.
+    exists (I ++ [i]); split; last set_solver.
+    eapply pool_steps_trans; eauto. eapply pool_steps_single.
+    rewrite -(list_insert_insert T i e'' e').
+    eapply prim_step_pool_step; first done.
+    eapply list_lookup_insert, lookup_lt_Some, Hlook.
+  Qed.
+
+  Lemma pool_reach_stuck_no_forks π p T e e' σ σ':
+    T !! π = Some e →
+    steps_no_fork p e σ e' σ' → pool_reach_stuck p (<[π := e']>T) σ' → pool_reach_stuck p T σ.
+  Proof.
+    intros HT Hnfs Hrs.
+    pose proof no_forks_pool_steps _ _ _ _ _ _ _ Hnfs HT as [? [??]].
+    by apply: pool_steps_reach_stuck.
+  Qed.
+
+  Lemma pool_safe_no_forks p T e σ i e' σ':
+    pool_safe p T σ →
+    T !! i = Some e →
+    steps_no_fork p e σ e' σ' →
+    pool_safe p (<[i := e']>T) σ'.
+  Proof.
+    intros Hsafe HT Hnfs.
+    pose proof no_forks_pool_steps _ _ _ _ _ _ _ Hnfs HT as [? [??]].
+    by apply: pool_steps_safe.
+  Qed.
+
+  Lemma safe_call_in_prg p K e σ σ' f vs:
+    safe p e σ →
+    steps_no_fork p e σ (fill K (of_call f vs)) σ' →
+    ∃ fn, p !! f = Some fn.
+  Proof.
+    intros H1 (I & Hsteps)%no_forks_pool_steps_single_thread.
+    eapply (pool_safe_call_in_prg _ _ _ _ 0) in Hsteps; eauto.
+  Qed.
+
+  Lemma no_forks_val p v σ e' σ' :
+    steps_no_fork p (of_val v) σ e' σ' → e' = of_val v ∧ σ' = σ.
+  Proof.
+    intros (I & Hsteps)%no_forks_pool_steps_single_thread.
+    eapply pool_steps_values in Hsteps; first naive_solver.
+    intros e Hel. assert (e = of_val v) as -> by set_solver.
+    rewrite to_of_val; eauto.
+  Qed.
+
+  Lemma val_safe p v σ : safe p (of_val v) σ.
+  Proof.
+    intros T' σ' I Hsteps e i Hlookup.
+    eapply pool_steps_values in Hsteps as (-> & -> & ->); last first.
+    { intros e' Hel. assert (e' = of_val v) as -> by set_solver.
+      rewrite to_of_val; eauto. }
+    rewrite list_lookup_singleton in Hlookup. destruct i; last done.
+    assert (e = of_val v) as -> by congruence.
+    left. rewrite to_of_val. eauto.
+  Qed.
+
+  Lemma reach_stuck_no_forks P e σ e' σ':
+    reach_stuck P e' σ' → steps_no_fork P e σ e' σ' →  reach_stuck P e σ.
+  Proof.
+    intros (T'' & σ'' & I & Hsteps & Hstuck) (J & Hnfs)%no_forks_pool_steps_single_thread.
+    exists T'', σ'', (J ++ I). split; last done.
+    by eapply pool_steps_trans.
+  Qed.
+
+  Lemma safe_no_forks P e σ e' σ':
+    safe P e σ → steps_no_fork P e σ e' σ' → safe P e' σ'.
+  Proof.
+    intros Hsafe (J & Hnfs)%no_forks_pool_steps_single_thread T'' σ'' I Hsteps e'' i Hlookup.
+    eapply Hsafe. { eapply pool_steps_trans; done. }
+    done.
+  Qed.
+
+  Lemma no_forks_trans P e σ e' σ' e'' σ'':
+    steps_no_fork P e σ e' σ' → steps_no_fork P e' σ' e'' σ'' → steps_no_fork P e σ e'' σ''.
+  Proof.
+    induction 1; eauto using steps_no_fork.
+  Qed.
+
+  Lemma no_forks_inv_r P e σ e' σ':
+    steps_no_fork P e σ e' σ' → (e' = e ∧ σ' = σ) ∨ (∃ e'' σ'', steps_no_fork P e σ e'' σ'' ∧ step_no_fork P e'' σ'' e' σ').
+  Proof.
+    induction 1 as [|e e' e'' σ σ' σ'' Hstep Hsteps IH]; first by eauto.
+    destruct IH as [(-> & ->)|(e''' & σ''' & Hnfs & Hnf)]; eauto 10 using steps_no_fork.
+  Qed.
+
+End language.
+
+
+Section safe_reach.
+  Context {Λ : language}.
+
+  (** [post_in_ectx] allows ignoring arbitrary evaluation contexts
+  around e and is meant as a combinator for the postcondition of
+  [safe_reach]. *)
+  Definition post_in_ectx (Φ : expr Λ → state Λ → Prop) (e : expr Λ) (σ : state Λ) : Prop :=
+    ∃ Ks e', e = fill Ks e' ∧ Φ e' σ.
+
+  Lemma post_in_ectx_intro (Φ : expr Λ → state Λ → Prop) e σ:
+    Φ e σ →
+    post_in_ectx Φ e σ.
+  Proof. eexists empty_ectx, e. rewrite fill_empty. naive_solver. Qed.
+
+  Lemma post_in_ectx_mono (Φ1 Φ2 : expr Λ → state Λ → Prop) e σ:
+    post_in_ectx Φ1 e σ →
+    (∀ e σ, Φ1 e σ → Φ2 e σ) →
+    post_in_ectx Φ2 e σ.
+  Proof. move => [?[?[??]]] ?. eexists _, _. naive_solver. Qed.
+
+  (** [safe_reach P e σ Φ] says that starting from e in state σ,
+    under the assumption that this is a [safe] configuration,
+     one can reach e' in σ' such that Φ e' σ' holds. *)
+  Definition safe_reach (P : prog Λ) (e : expr Λ) (σ : state Λ) (Φ : expr Λ → state Λ → Prop) : Prop :=
+    safe P e σ → ∃ e' σ', steps_no_fork P e σ e' σ' ∧ Φ e' σ'.
+
+  Lemma safe_reach_refl p e σ (Φ : _ → _ → Prop):
+    Φ e σ → safe_reach p e σ Φ.
+  Proof. move => ? ?. eexists _, _ => /=. split; [|done]. by apply: no_forks_refl. Qed.
+
+  Lemma safe_reach_mono p e σ (Φ1 Φ2 : _ → _ → Prop):
+    safe_reach p e σ Φ1 → (∀ e σ, Φ1 e σ → Φ2 e σ) → safe_reach p e σ Φ2.
+  Proof. intros Hsr ? (? & ? & ? & ?)%Hsr. eexists _, _. naive_solver. Qed.
+
+  Lemma safe_reach_no_forks p e σ e' σ' (Φ : _ → _ → Prop):
+    steps_no_fork p e σ e' σ' → safe_reach p e' σ' Φ → safe_reach p e σ Φ.
+  Proof.
+    intros Hsteps Hsr Hsafe. specialize (safe_no_forks _ _ _ _ _ Hsafe Hsteps) as (?&?&?&?)%Hsr.
+    eexists _, _. split; last done. by apply: no_forks_trans.
+  Qed.
+
+  Lemma safe_reach_step p e σ e' σ' (Φ : _ → _ → Prop):
+    prim_step p e σ e' σ' [] → safe_reach p e' σ' Φ → safe_reach p e σ Φ.
+  Proof.
+    move => ??. apply: safe_reach_no_forks; [|done].
+    apply: no_forks_step; [done|]. apply: no_forks_refl.
+  Qed.
+
+  Lemma safe_reach_head_step p e σ e' σ' (Φ : _ → _ → Prop):
+    head_step p e σ e' σ' [] → safe_reach p e' σ' Φ → safe_reach p e σ Φ.
+  Proof. move => ??. apply: safe_reach_step; [|done]. by apply: head_prim_step. Qed.
+
+  Lemma fill_safe_reach p e σ Φ Ks:
+    safe_reach p e σ (post_in_ectx Φ) → safe_reach p (fill Ks e) σ (post_in_ectx Φ).
+  Proof.
+    intros Hsr (?&?&?&Hp)%fill_safe%Hsr.
+    eexists _, _. split; [ by apply: fill_no_forks | ].
+    destruct Hp as (? & ? & -> & ?).
+    eexists _, _. rewrite fill_comp. naive_solver.
+  Qed.
+
+  Lemma safe_reach_bind p e σ Φ Ks:
+    safe_reach p e σ (λ e' σ', safe_reach p (fill Ks e') σ' Φ) → safe_reach p (fill Ks e) σ Φ.
+  Proof.
+    intros Hsr Hsafe.
+    specialize (Hsr (fill_safe _ _ _ _  Hsafe)) as (? &?&?&Hp).
+    destruct Hp as (?&?& ? & ?).
+    { eapply safe_no_forks; first done. by apply fill_no_forks. }
+    eexists _, _. split; last done.
+    eapply no_forks_trans.
+    - by eapply fill_no_forks.
+    - done.
+  Qed.
+
+  Lemma pool_safe_safe_reach π p T e σ Φ K:
+    pool_safe p T σ →
+    T !! π = Some (fill K e) →
+    safe_reach p e σ Φ →
+    ∃ e' σ',  Φ e' σ' ∧ pool_safe p (<[π := fill K e']>T) σ'.
+  Proof.
+    intros Hs Hlook Hsr.
+    assert (safe p e σ) as (e' & σ' & ? & ?)%Hsr.
+    { eapply fill_safe. eapply pool_safe_threads_safe; done. }
+    eexists _, _. split; first done.
+    eapply pool_safe_no_forks; [done..|]. by apply: fill_no_forks.
+  Qed.
+
+  Lemma pool_safe_safe_reach_stuck π p T e σ Φ :
+    pool_safe p T σ →
+    T !! π = Some e →
+    safe_reach p e σ Φ →
+    (∀ e' σ', Φ e' σ' → pool_safe p (<[π := e']> T) σ' → pool_reach_stuck p (<[π := e']>T) σ') →
+    pool_reach_stuck p T σ.
+  Proof.
+    intros Hs Hlook Hsr Hp. edestruct Hsr as (e' & σ' & Hsteps & Hphi).
+    { by eapply pool_safe_threads_safe. }
+    apply Hp in Hphi.
+    - eapply pool_reach_stuck_no_forks; done.
+    - eapply pool_safe_no_forks; done.
+  Qed.
+End safe_reach.
+
+
+(* discrete OFE instance for expr and thread_id *)
+Definition exprO {Λ : language} := leibnizO (expr Λ).
+Global Instance expr_equiv {Λ} : Equiv (expr Λ). apply exprO. Defined.
+
+Definition thread_idO := leibnizO thread_id.
+Global Instance thread_id_equiv : Equiv thread_id. apply thread_idO. Defined.
